src/Eqvivalence/Basics.v
@@ -1,0 +1,147 @@
+From CoreErlang.Eqvivalence.Tactics Require Export T1ParamZero.
+From CoreErlang.Eqvivalence.Tactics Require Export T2ParamSingle.
+From CoreErlang.Eqvivalence.Tactics Require Export T3ParamMultiple.
+From CoreErlang.Eqvivalence.Tactics Require Export T4Name.
+From CoreErlang.Eqvivalence.Tactics Require Export T5Transform.
+From CoreErlang.Eqvivalence Require Export Induction.
+From CoreErlang.Eqvivalence Require Export WellFormedMap.
+From CoreErlang Require Export Basics.
+From CoreErlang.BigStep Require Export BigStep.
+From CoreErlang.FrameStack Require Export SubstSemanticsLemmas.
+Require Export stdpp.list.
+
+(* STRUCTURE:
+* Lists
+  - length_lt_split
+  - cons_app
+* Zips
+  - zip_fst
+  - zip_snd
+* Extensions
+  - ext_to_env_fst
+*)
+
+
+
+
+
+
+
+
+
+
+
+
+Section Lists.
+
+
+
+  Lemma cons_app :
+    forall T (x : T) (l : list T),
+      x :: l = [x] ++ l.
+  Proof.
+    trv.
+  Qed.
+
+
+
+  Lemma length_lt_split :
+    forall A B (al : list A) (bl : list B),
+        length al < length bl
+    ->  exists bl1 bl2 : list B,
+            bl = bl1 ++ bl2
+        /\  length bl1 = length al.
+  Proof.
+    (* #1 Exists: intro/exists/split *)
+    itr - A B al bl Hl.
+    exi - (firstn (length al) bl)
+          (skipn (length al) bl).
+    spl.
+    * (* #2.1 Equality: rewrite *)
+      by rewrite take_drop.
+    * (* #2.2 Length: rewrite/reflexivity/lia *)
+      rwr - firstn_length_le.
+      - rfl.
+      - lia.
+  Qed.
+
+
+
+End Lists.
+
+
+
+
+
+
+
+
+
+Section Zips.
+
+
+
+  Lemma zip_fst :
+    forall A B (al : list A) (bl : list B),
+    	length al = length bl
+    ->  map fst (zip al bl) = al.
+  Proof.
+    itr - A B al bl Hlen_eq.
+    ass > (length al <= length bl) as Hlen_le: lia.
+    apply fst_zip.
+    asm.
+  Qed.
+
+
+
+  Lemma zip_snd :
+    forall A B (al : list A) (bl : list B),
+    	length al = length bl
+    ->  map snd (zip al bl) = bl.
+  Proof.
+    itr - A B al bl Hlen_eq.
+    ass > (length bl <= length al) as Hlen_le: lia.
+    apply snd_zip.
+    asm.
+  Qed.
+
+
+
+End Zips.
+
+
+
+
+
+
+
+
+
+Section Extension.
+
+  Import BigStep.
+
+
+
+  Lemma ext_to_env_fst :
+    forall ext defext Γ,
+      map
+        fst
+        (map
+          (fun '(n, fid, (vars, e)) =>
+            (inr fid : (Var + FunctionIdentifier), VClos Γ defext n vars e))
+          ext)
+    = map (inr ∘ snd ∘ fst) ext.
+  Proof.
+    itr - ext.
+    ind - ext as [| [[n fid] [vars e]] ext IH]: smp.
+    itr - defext Γ.
+    smp.
+    feq.
+    spe - IH: defext Γ.
+    exa - IH.
+  Qed.
+
+
+
+End Extension.
