src/Eqvivalence/BsFs/Eqvivalence.v
@@ -1,0 +1,1724 @@
+From CoreErlang.Eqvivalence.BsFs Require Import Helpers.
+
+Import BigStep.
+
+(** CONTENT:
+* EQBSFS_ATOMS (LEMMAS)
+  - Nil
+  - Lit
+* EQBSFS_REFERENCES (LEMMAS)
+  - Var
+  - FunId
+* EQBSFS_SEQUENCES (LEMMAS)
+  - Cons
+  - Seq
+* EQBSFS_FUNCTIONS (LEMMAS)
+  - Fun
+  - LetRec
+* EQBSFS_BINDERS (LEMMAS)
+  - Let
+  - Try
+* EQBSFS_LISTS (LEMMAS)
+  - Values
+  - Tuple
+  - Map
+* EQBSFS_ COMPOUNDS (LEMMAS)
+  - PrimOp
+  - Apply
+  - Call
+  - Case
+* EQBSFS_ COMPOUNDS (LEMMAS)
+  - Main
+*)
+
+(* 
+Search nat "comm".
+
+
+  Ltac mred_le_solver2 :=
+    smp;
+    try unfold measure_val_list;
+    try unfold measure_val_map;
+    try unfold measure_val_env;
+    try rewrite map_app, list_sum_app;
+    (sli + (rewrite Nat.add_comm; slia)).
+
+Ltac mred2 :=
+    try (rewrite mred_min; [idtac | mred_le_solver]);
+    try (rewrite mred_min_list; [idtac | mred_le_solver]);
+    try (rewrite mred_min_map; [idtac | mred_le_solver]).
+
+Ltac mred2_all :=
+  repeat (
+    mred2;
+    try (rewrite mred_min; [idtac | mred_le_solver2]);
+    try (rewrite mred_min_list; [idtac | mred_le_solver2]);
+    try (rewrite mred_min_map; [idtac | mred_le_solver2])
+  ).
+
+
+Theorem eq_bsfs :
+  forall Γ modules own_module id id' e e' eff eff' σ,
+      (eval_expr Γ modules own_module id e eff id' e' eff')
+  ->  ⟨ [], (erase_names σ Γ e) ⟩ -->* erase_result σ e'.
+Proof.
+  itr - Γ modules own_module id id' e e' eff eff' σ B.
+  gen - σ.
+  ind - B; itr.
+  10: {
+    smp.
+    assert ((erase_val (measure_val hdv + measure_val tlv) σ hdv) = (erase_val (measure_val hdv) σ hdv)).
+    apply measure_reduction.
+    mred2_all.
+    mred2.
+    rewrite mred_min with (v := tlv).
+    eei; spl.
+    admit.
+    ens.
+    cns.
+    mred2.
+    ens.
+    
+    do 5 mred2.
+    rewrite mred_min.
+  }
+Admitted. *)
+
+
+
+
+
+
+
+
+(*
+////////////////////////////////////////////////////////////////////////////////
+//// EQBSFS_ATOMS //////////////////////////////////////////////////////////////
+////////////////////////////////////////////////////////////////////////////////
+*)
+
+
+
+
+
+
+Section ENil.
+
+
+
+  Theorem eq_bsfs_enil :
+    forall Γ σ,
+      ⟨ [], erase_names σ Γ ENil ⟩
+        -->*
+      erase_result σ (inl [VNil]).
+  Proof.
+    itr.
+    smp.
+    start.
+    step.
+  Qed.
+
+
+
+End ENil.
+
+
+
+
+
+
+
+
+
+Section ELit.
+
+
+
+  Theorem eq_bsfs_elit :
+    forall lit Γ σ,
+      ⟨ [], erase_names σ Γ (ELit lit) ⟩
+        -->*
+      erase_result σ (inl [VLit lit]).
+  Proof.
+    itr.
+    smp.
+    start.
+    step.
+  Qed.
+
+
+
+End ELit.
+
+
+
+
+
+
+
+
+
+
+
+
+(*
+////////////////////////////////////////////////////////////////////////////////
+//// EQBSFS_REFERENCES /////////////////////////////////////////////////////////
+////////////////////////////////////////////////////////////////////////////////
+*)
+
+Section tmp.
+
+(*
+
+
+env : Environment
+modules : list ErlModule
+own_module : string
+s : Var
+eff : SideEffectList
+id : nat
+res : ValueSequence
+H : get_value env (inl s) = Some res
+σ : NameSub
+______________________________________(1/1)
+⟨ [], erase_names σ env (EVar s) ⟩ -->* erase_result σ (inl res)
+
+*)
+
+
+
+End tmp.
+
+Section tmp.
+
+(*
+
+env : Environment
+modules : list ErlModule
+own_module : string
+fid : FunctionIdentifier
+eff : SideEffectList
+res : ValueSequence
+id : nat
+H : get_value env (inr fid) = Some res
+σ : NameSub
+______________________________________(1/1)
+⟨ [], erase_names σ env (EFunId fid) ⟩ -->* erase_result σ (inl res)
+
+
+
+
+env : Environment
+modules : list ErlModule
+own_module : string
+fid : FunctionIdentifier
+eff : SideEffectList
+func : TopLevelFunction
+body_func : Expression
+varl_func : list Var
+id : nat
+H : get_value env (inr fid) = None
+H0 : get_own_modfunc own_module fid.1 fid.2 (modules ++ stdlib) = Some func
+H1 : varl_func = varl func
+H2 : body_func = body func
+σ : NameSub
+______________________________________(1/1)
+⟨ [], erase_names σ env (EFunId fid) ⟩ -->*
+erase_result σ (inl [VClos env [] id varl_func body_func])
+
+*)
+
+
+
+End tmp.
+
+
+
+
+
+
+
+
+
+
+
+
+(*
+////////////////////////////////////////////////////////////////////////////////
+//// EQBSFS_SEQUENCES //////////////////////////////////////////////////////////
+////////////////////////////////////////////////////////////////////////////////
+*)
+
+
+
+
+
+
+Section ECons.
+
+
+
+  Theorem eq_bsfs_econs :
+    forall e1 e2 v1 v2 Γ σ,
+        (forall σ,
+          ⟨ [], erase_names σ Γ e1 ⟩
+            -->*
+          erase_result σ (inl [v1]))
+    ->  (forall σ,
+          ⟨ [], erase_names σ Γ e2 ⟩
+            -->*
+          erase_result σ (inl [v2]))
+    ->  ⟨ [], erase_names σ Γ (ECons e1 e2) ⟩
+          -->*
+        erase_result σ (inl [VCons v1 v2]).
+  Proof.
+    itr - e1 e2 v1 v2 Γ σ IHv1 IHv2.
+    (* #1 Simplify: simpl/unfold *)
+    smp *.
+    ufl - erase_names in *.
+    (* #2 Specialize Inductive Hypothesis: specialize *)
+    spe - IHv1: σ.
+    spe - IHv2: σ.
+    (* #3 Measure Reduction & Remember: remember/clear/measure_reduction *)
+    rem - subst' as Hsubst:
+      (list_subst
+        (map
+          (λ v : Value, erase_val (measure_val v) σ v)
+          (map snd Γ))
+        idsubst).
+    clr - Hsubst.
+    mred.
+    rem - e1' v1' as He1 Hv1:
+      (erase_exp (add_keys (map fst Γ) σ) e1)
+      (erase_val (measure_val v1) σ v1).
+    clr - He1 e1.
+    mred.
+    rem - e2' v2' as He2 Hv2:
+      (erase_exp (add_keys (map fst Γ) σ) e2)
+      (erase_val (measure_val v2) σ v2).
+    clr - He2 e2.
+    clr - Hv1 v1 Hv2 v2.
+    clr - Γ σ.
+    (* #4 Destruct Inductive Hypothesis: destruct *)
+    des - IHv1 as [kv1 [Hscope_v1 Hstep_v1]].
+    des - IHv2 as [kv2 [Hscope_v2 Hstep_v2]].
+    (* #5 Scope & Step: start/step *)
+    start / Hscope_v1 Hscope_v2.
+    step - Hstep_v2 / e2' kv2.
+    step - Hstep_v1 / e1' kv1 subst'.
+    step.
+  Qed.
+
+
+
+  Theorem eq_bsfs_econs_exc1 :
+    forall e1 e2 exc v2 Γ σ,
+        (forall σ,
+          ⟨ [], erase_names σ Γ e1 ⟩
+            -->*
+          erase_result σ (inr exc))
+    ->  (forall σ,
+          ⟨ [], erase_names σ Γ e2 ⟩
+            -->*
+          erase_result σ (inl [v2]))
+    ->  ⟨ [], erase_names σ Γ (ECons e1 e2) ⟩
+          -->*
+        erase_result σ (inr exc).
+  Proof.
+    itr - e1 e2 exc v2 Γ σ IHexc IHv2.
+    (* #1 Simplify: simpl/unfold *)
+    smp *.
+    ufl - erase_names in *.
+    (* #2 Specialize Inductive Hypothesis: specialize *)
+    spe - IHexc: σ.
+    spe - IHv2: σ.
+    (* #3 Measure Reduction & Remember: remember/clear/measure_reduction *)
+    rem - subst' as Hsubst:
+      (list_subst
+        (map
+          (λ v : Value, erase_val (measure_val v) σ v)
+          (map snd Γ))
+        idsubst).
+    clr - Hsubst.
+    mred.
+    rem - e1' exc' as He1 Hexc:
+      (erase_exp (add_keys (map fst Γ) σ) e1)
+      (erase_exc σ exc).
+    clr - He1 e1.
+    mred.
+    rem - e2' v2' as He2 Hv2:
+      (erase_exp (add_keys (map fst Γ) σ) e2)
+      (erase_val (measure_val v2) σ v2).
+    clr - He2 e2.
+    clr - Hexc exc Hv2 v2.
+    clr - Γ σ.
+    (* #4 Destruct Inductive Hypothesis: destruct *)
+    des - IHexc as [kexc [Hscope_exc Hstep_exc]].
+    des - IHv2 as [kv2 [_ Hstep_v2]].
+    (* #5 Scope & Step: start/step *)
+    start / Hscope_exc.
+    step - Hstep_v2 / e2' kv2.
+    step - Hstep_exc / e1' kexc subst'.
+    step.
+  Qed.
+
+
+
+  Theorem eq_bsfs_econs_exc2 :
+    forall e1 e2 exc Γ σ,
+        (forall σ,
+          ⟨ [], erase_names σ Γ e2 ⟩
+            -->*
+          erase_result σ (inr exc))
+    ->  ⟨ [], erase_names σ Γ (ECons e1 e2) ⟩
+          -->*
+        erase_result σ (inr exc).
+  Proof.
+    itr - e1 e2 exc Γ σ IHexc.
+    (* #1 Simplify: simpl/unfold *)
+    smp *.
+    ufl - erase_names in *.
+    (* #2 Specialize Inductive Hypothesis: specialize *)
+    spe - IHexc: σ.
+    (* #3 Measure Reduction & Remember: remember/clear/measure_reduction *)
+    rem - subst' as Hsubst:
+      (list_subst
+        (map
+          (λ v : Value, erase_val (measure_val v) σ v)
+          (map snd Γ))
+        idsubst).
+    clr - Hsubst.
+    mred.
+    rem - e1' exc' as He1 Hexc:
+      (erase_exp (add_keys (map fst Γ) σ) e1)
+      (erase_exc σ exc).
+    clr - He1 e1.
+    mred.
+    rem - e2' as He2:
+      (erase_exp (add_keys (map fst Γ) σ) e2).
+    clr - He2 e2.
+    clr - Hexc exc.
+    clr - Γ σ.
+    (* #4 Destruct Inductive Hypothesis: destruct *)
+    des - IHexc as [kexc [Hscope_exc Hstep_exc]].
+    (* #5 Scope & Step: start/step *)
+    start / Hscope_exc.
+    step - Hstep_exc / kexc.
+    step.
+  Qed.
+
+
+
+End ECons.
+
+
+
+
+
+
+
+
+
+Section ESeq.
+
+
+
+  Theorem eq_bsfs_eseq :
+    forall e1 e2 v1 v2 Γ σ,
+        (forall σ,
+          ⟨ [], erase_names σ Γ e1 ⟩
+            -->*
+          erase_result σ (inl [v1]))
+    ->  (forall σ,
+          ⟨ [], erase_names σ Γ e2 ⟩
+            -->*
+          erase_result σ (inl v2))
+    ->  ⟨ [], erase_names σ Γ (ESeq e1 e2) ⟩
+          -->*
+        erase_result σ (inl v2).
+  Proof.
+    itr - e1 e2 v1 v2 Γ σ IHv1 IHv2.
+    (* #1 Simplify: simpl/unfold *)
+    smp *.
+    ufl - erase_names in *.
+    (* #2 Specialize Inductive Hypothesis: specialize *)
+    spe - IHv1: σ.
+    spe - IHv2: σ.
+    (* #3 Measure Reduction & Remember: remember/clear/measure_reduction *)
+    rem - subst' as Hsubst:
+      (list_subst
+        (map
+          (λ v : Value, erase_val (measure_val v) σ v)
+          (map snd Γ))
+        idsubst).
+    clr - Hsubst.
+    mred.
+    rem - e1' v1' as He1 Hv1:
+      (erase_exp (add_keys (map fst Γ) σ) e1)
+      (erase_val (measure_val v1) σ v1).
+    clr - He1 e1.
+    mred.
+    rem - e2' v2' as He2 Hv2:
+      (erase_exp (add_keys (map fst Γ) σ) e2)
+      (map (λ v : Value, erase_val (measure_val v) σ v) v2).
+    clr - He2 e2.
+    clr - Hv1 v1 Hv2 v2.
+    clr - Γ σ.
+    (* #4 Destruct Inductive Hypothesis: destruct *)
+    des - IHv1 as [kv1 [_ Hstep_v1]].
+    des - IHv2 as [kv2 [Hscope_v2 Hstep_v2]].
+    (* #5 Scope & Step: start/step *)
+    start - Hscope_v2.
+    step - Hstep_v1 / e1' kv1.
+    step - Hstep_v2.
+  Qed.
+
+
+
+  Theorem eq_bsfs_eseq_exc :
+    forall e1 e2 exc Γ σ,
+        (forall σ,
+          ⟨ [], erase_names σ Γ e1 ⟩
+            -->*
+          erase_result σ (inr exc))
+    ->  ⟨ [], erase_names σ Γ (ESeq e1 e2) ⟩
+          -->*
+        erase_result σ (inr exc).
+  Proof.
+    itr - e1 e2 exc Γ σ IHexc.
+    (* #1 Simplify: simpl/unfold *)
+    smp *.
+    ufl - erase_names in *.
+    (* #2 Specialize Inductive Hypothesis: specialize *)
+    spe - IHexc: σ.
+    (* #3 Measure Reduction & Remember: remember/clear/measure_reduction *)
+    rem - subst' as Hsubst:
+      (list_subst
+        (map
+          (λ v : Value, erase_val (measure_val v) σ v)
+          (map snd Γ))
+        idsubst).
+    clr - Hsubst.
+    mred.
+    rem - e1' exc' as He1 Hexc:
+      (erase_exp (add_keys (map fst Γ) σ) e1)
+      (erase_exc σ exc).
+    clr - He1 e1.
+    mred.
+    rem - e2' as He2:
+      (erase_exp (add_keys (map fst Γ) σ) e2).
+    clr - He2 e2.
+    clr - Hexc exc.
+    clr - Γ σ.
+    (* #4 Destruct Inductive Hypothesis: destruct *)
+    des - IHexc as [kexc [Hscope_exc Hstep_exc]].
+    (* #5 Scope & Step: start/step *)
+    start / Hscope_exc.
+    step - Hstep_exc / e1' kexc.
+    step.
+  Qed.
+
+
+
+End ESeq.
+
+
+
+
+
+
+
+
+
+
+
+
+(*
+////////////////////////////////////////////////////////////////////////////////
+//// EQBSFS_FUNCTIONS //////////////////////////////////////////////////////////
+////////////////////////////////////////////////////////////////////////////////
+*)
+
+Section tmp.
+
+(*
+
+env : Environment
+modules : list ErlModule
+own_module : string
+vl : list Var
+e : Expression
+eff : SideEffectList
+id : nat
+σ : NameSub
+______________________________________(1/1)
+⟨ [], erase_names σ env (EFun vl e) ⟩ -->* erase_result σ (inl [VClos env [] id vl e])
+
+*)
+
+
+
+End tmp.
+
+Section tmp.
+
+(*
+
+env : Environment
+modules : list ErlModule
+own_module : string
+e : Expression
+l : list (FunctionIdentifier * (list Var * Expression))
+res : ValueSequence + Exception
+eff1, eff2 : SideEffectList
+id, id' : nat
+B :
+  | append_funs_to_env l env id, modules, own_module, id + base.length l, e, eff1 | -e> | id', res,
+  eff2 |
+IHB : ∀ σ : NameSub, ⟨ [], erase_names σ (append_funs_to_env l env id) e ⟩ -->* erase_result σ res
+σ : NameSub
+______________________________________(1/1)
+⟨ [], erase_names σ env (ELetRec l e) ⟩ -->* erase_result σ res
+
+*)
+
+
+
+End tmp.
+
+
+
+
+
+
+
+
+
+
+
+
+(*
+////////////////////////////////////////////////////////////////////////////////
+//// EQBSFS_BINDERS ////////////////////////////////////////////////////////////
+////////////////////////////////////////////////////////////////////////////////
+*)
+
+Section tmp.
+
+(*
+
+env : Environment
+modules : list ErlModule
+own_module : string
+l : list Var
+vals : ValueSequence
+e1, e2 : Expression
+res : ValueSequence + Exception
+eff1, eff', eff'' : SideEffectList
+id, id', id'' : nat
+B1 : | env, modules, own_module, id, e1, eff1 | -e> | id', inl vals, eff' |
+H : base.length l = base.length vals
+B2 : | append_vars_to_env l vals env, modules, own_module, id', e2, eff' | -e> | id'', res, eff'' |
+IHB1 : ∀ σ : NameSub, ⟨ [], erase_names σ env e1 ⟩ -->* erase_result σ (inl vals)
+IHB2 :
+  ∀ σ : NameSub, ⟨ [], erase_names σ (append_vars_to_env l vals env) e2 ⟩ -->* erase_result σ res
+σ : NameSub
+______________________________________(1/1)
+⟨ [], erase_names σ env (ELet l e1 e2) ⟩ -->* erase_result σ res
+
+
+
+
+env : Environment
+modules : list ErlModule
+own_module : string
+vl : list Var
+e1, e2 : Expression
+ex : Exception
+eff1, eff2 : SideEffectList
+id, id' : nat
+B : | env, modules, own_module, id, e1, eff1 | -e> | id', inr ex, eff2 |
+IHB : ∀ σ : NameSub, ⟨ [], erase_names σ env e1 ⟩ -->* erase_result σ (inr ex)
+σ : NameSub
+______________________________________(1/1)
+⟨ [], erase_names σ env (ELet vl e1 e2) ⟩ -->* erase_result σ (inr ex)
+
+
+
+*)
+
+
+
+End tmp.
+
+Section tmp.
+
+(*
+
+env : Environment
+modules : list ErlModule
+own_module : string
+vl1, vl2 : list Var
+e1, e2, e3 : Expression
+res : ValueSequence + Exception
+vals : ValueSequence
+eff1, eff2, eff3 : SideEffectList
+id, id', id'' : nat
+B1 : | env, modules, own_module, id, e1, eff1 | -e> | id', inl vals, eff2 |
+H : base.length vl1 = base.length vals
+B2 : | append_vars_to_env vl1 vals env, modules, own_module, id', e2, eff2 | -e> | id'', res, eff3 |
+IHB1 : ∀ σ : NameSub, ⟨ [], erase_names σ env e1 ⟩ -->* erase_result σ (inl vals)
+IHB2 :
+  ∀ σ : NameSub, ⟨ [], erase_names σ (append_vars_to_env vl1 vals env) e2 ⟩ -->* erase_result σ res
+σ : NameSub
+______________________________________(1/1)
+⟨ [], erase_names σ env (ETry e1 vl1 e2 vl2 e3) ⟩ -->* erase_result σ res
+
+
+
+
+env : Environment
+modules : list ErlModule
+own_module : string
+vl1, vl2 : list Var
+e1, e2, e3 : Expression
+res : ValueSequence + Exception
+eff1, eff2, eff3 : SideEffectList
+id, id', id'' : nat
+ex : Exception
+B1 : | env, modules, own_module, id, e1, eff1 | -e> | id', inr ex, eff2 |
+B2 :
+  | append_try_vars_to_env vl2 [exclass_to_value ex.1.1; ex.1.2; ex.2] env, modules, own_module,
+  id', e3, eff2 | -e> | id'', res, eff3 |
+IHB1 : ∀ σ : NameSub, ⟨ [], erase_names σ env e1 ⟩ -->* erase_result σ (inr ex)
+IHB2 :
+  ∀ σ : NameSub,
+    ⟨ [], erase_names σ (append_try_vars_to_env vl2 [exclass_to_value ex.1.1; ex.1.2; ex.2] env) e3
+    ⟩ -->* erase_result σ res
+σ : NameSub
+______________________________________(1/1)
+⟨ [], erase_names σ env (ETry e1 vl1 e2 vl2 e3) ⟩ -->* erase_result σ res
+
+
+*)
+
+
+
+End tmp.
+
+
+
+
+
+
+
+
+
+
+
+
+(*
+////////////////////////////////////////////////////////////////////////////////
+//// EQBSFS_LISTS //////////////////////////////////////////////////////////////
+////////////////////////////////////////////////////////////////////////////////
+*)
+
+Section tmp.
+
+(*
+
+env : Environment
+modules : list ErlModule
+own_module : string
+exps : list Expression
+vals : list Value
+eff : list (list (SideEffectId * list Value))
+ids : list nat
+eff1 : list (SideEffectId * list Value)
+id : nat
+eff' : list (SideEffectId * list Value)
+id' : nat
+H : base.length exps = base.length vals
+H0 : base.length exps = base.length eff
+H1 : base.length exps = base.length ids
+H2 :
+  ∀ i : nat,
+    i < base.length exps
+    → | env, modules, own_module, nth_def ids id 0 i, nth i exps ErrorExp, 
+      nth_def eff eff1 [] i | -e> | nth_def ids id 0 (S i), inl [nth i vals ErrorValue],
+      nth_def eff eff1 [] (S i) |
+H3 :
+  ∀ i : nat,
+    i < base.length exps
+    → ∀ σ : NameSub,
+        ⟨ [], erase_names σ env (nth i exps ErrorExp) ⟩ -->*
+        erase_result σ (inl [nth i vals ErrorValue])
+H4 : id' = last ids id
+H5 : eff' = last eff eff1
+σ : NameSub
+______________________________________(1/1)
+⟨ [], erase_names σ env (EValues exps) ⟩ -->* erase_result σ (inl vals)
+
+
+
+
+
+env : Environment
+modules : list ErlModule
+own_module : string
+exps : list Expression
+ex : Exception
+vals : list Value
+eff : list (list (SideEffectId * list Value))
+ids : list nat
+eff1 : list (SideEffectId * list Value)
+id : nat
+eff' : SideEffectList
+id', i : nat
+H : i < base.length exps
+H0 : base.length vals = i
+H1 : base.length eff = i
+H2 : base.length ids = i
+H3 :
+  ∀ j : nat,
+    j < i
+    → | env, modules, own_module, nth_def ids id 0 j, nth j exps ErrorExp, 
+      nth_def eff eff1 [] j | -e> | nth_def ids id 0 (S j), inl [nth j vals ErrorValue],
+      nth_def eff eff1 [] (S j) |
+H4 :
+  ∀ j : nat,
+    j < i
+    → ∀ σ : NameSub,
+        ⟨ [], erase_names σ env (nth j exps ErrorExp) ⟩ -->*
+        erase_result σ (inl [nth j vals ErrorValue])
+B :
+  | env, modules, own_module, last ids id, nth i exps ErrorExp, last eff eff1 | -e> | id', 
+  inr ex, eff' |
+IHB : ∀ σ : NameSub, ⟨ [], erase_names σ env (nth i exps ErrorExp) ⟩ -->* erase_result σ (inr ex)
+σ : NameSub
+______________________________________(1/1)
+⟨ [], erase_names σ env (EValues exps) ⟩ -->* erase_result σ (inr ex)
+
+
+
+*)
+
+
+
+End tmp.
+
+Section tmp.
+
+(*
+
+env : Environment
+modules : list ErlModule
+own_module : string
+exps : list Expression
+vals : list Value
+eff1, eff2 : SideEffectList
+eff : list SideEffectList
+ids : list nat
+id, id' : nat
+H : base.length exps = base.length vals
+H0 : base.length exps = base.length eff
+H1 : base.length exps = base.length ids
+H2 :
+  ∀ i : nat,
+    i < base.length exps
+    → | env, modules, own_module, nth_def ids id 0 i, nth i exps ErrorExp, 
+      nth_def eff eff1 [] i | -e> | nth_def ids id 0 (S i), inl [nth i vals ErrorValue],
+      nth_def eff eff1 [] (S i) |
+H3 :
+  ∀ i : nat,
+    i < base.length exps
+    → ∀ σ : NameSub,
+        ⟨ [], erase_names σ env (nth i exps ErrorExp) ⟩ -->*
+        erase_result σ (inl [nth i vals ErrorValue])
+H4 : eff2 = last eff eff1
+H5 : id' = last ids id
+σ : NameSub
+______________________________________(1/1)
+⟨ [], erase_names σ env (ETuple exps) ⟩ -->* erase_result σ (inl [VTuple vals])
+
+
+
+
+
+
+env : Environment
+modules : list ErlModule
+own_module : string
+i : nat
+exps : list Expression
+vals : list Value
+ex : Exception
+eff1, eff2 : SideEffectList
+eff : list SideEffectList
+id, id' : nat
+ids : list nat
+H : i < base.length exps
+H0 : base.length vals = i
+H1 : base.length eff = i
+H2 : base.length ids = i
+H3 :
+  ∀ j : nat,
+    j < i
+    → | env, modules, own_module, nth_def ids id 0 j, nth j exps ErrorExp, 
+      nth_def eff eff1 [] j | -e> | nth_def ids id 0 (S j), inl [nth j vals ErrorValue],
+      nth_def eff eff1 [] (S j) |
+H4 :
+  ∀ j : nat,
+    j < i
+    → ∀ σ : NameSub,
+        ⟨ [], erase_names σ env (nth j exps ErrorExp) ⟩ -->*
+        erase_result σ (inl [nth j vals ErrorValue])
+B :
+  | env, modules, own_module, last ids id, nth i exps ErrorExp, last eff eff1 | -e> | id', 
+  inr ex, eff2 |
+IHB : ∀ σ : NameSub, ⟨ [], erase_names σ env (nth i exps ErrorExp) ⟩ -->* erase_result σ (inr ex)
+σ : NameSub
+______________________________________(1/1)
+⟨ [], erase_names σ env (ETuple exps) ⟩ -->* erase_result σ (inr ex)
+
+
+*)
+
+
+
+End tmp.
+
+Section tmp.
+
+(*
+
+l : list (Expression * Expression)
+vvals, kvals, kvals', vvals' : list Value
+lv : list (Value * Value)
+env : Environment
+modules : list ErlModule
+own_module : string
+eff1, eff2 : SideEffectList
+eff : list SideEffectList
+ids : list nat
+id, id' : nat
+H : base.length l = base.length vvals
+H0 : base.length l = base.length kvals
+H1 : base.length l * 2 = base.length eff
+H2 : base.length l * 2 = base.length ids
+exps := make_map_exps l : list Expression
+vals := make_map_vals kvals vvals : list Value
+H3 :
+  ∀ i : nat,
+    i < base.length exps
+    → | env, modules, own_module, nth_def ids id 0 i, nth i exps ErrorExp, 
+      nth_def eff eff1 [] i | -e> | nth_def ids id 0 (S i), inl [nth i vals ErrorValue],
+      nth_def eff eff1 [] (S i) |
+H4 :
+  ∀ i : nat,
+    i < base.length exps
+    → ∀ σ : NameSub,
+        ⟨ [], erase_names σ env (nth i exps ErrorExp) ⟩ -->*
+        erase_result σ (inl [nth i vals ErrorValue])
+H5 : make_value_map kvals vvals = (kvals', vvals')
+H6 : combine kvals' vvals' = lv
+H7 : eff2 = last eff eff1
+H8 : id' = last ids id
+σ : NameSub
+______________________________________(1/1)
+⟨ [], erase_names σ env (EMap l) ⟩ -->* erase_result σ (inl [VMap lv])
+
+
+
+
+
+l : list (Expression * Expression)
+vvals, kvals : list Value
+env : Environment
+modules : list ErlModule
+own_module : string
+i : nat
+ex : Exception
+eff1, eff2 : SideEffectList
+eff : list SideEffectList
+ids : list nat
+id, id' : nat
+H : i < 2 * base.length l
+H0 : base.length vvals = i / 2
+H1 : base.length kvals = i / 2 + i mod 2
+H2 : base.length eff = i
+H3 : base.length ids = i
+exps := make_map_exps l : list Expression
+vals := make_map_vals kvals vvals : list Value
+H4 :
+  ∀ j : nat,
+    j < i
+    → | env, modules, own_module, nth_def ids id 0 j, nth j exps ErrorExp, 
+      nth_def eff eff1 [] j | -e> | nth_def ids id 0 (S j), inl [nth j vals ErrorValue],
+      nth_def eff eff1 [] (S j) |
+H5 :
+  ∀ j : nat,
+    j < i
+    → ∀ σ : NameSub,
+        ⟨ [], erase_names σ env (nth j exps ErrorExp) ⟩ -->*
+        erase_result σ (inl [nth j vals ErrorValue])
+B :
+  | env, modules, own_module, last ids id, nth i exps ErrorExp, last eff eff1 | -e> | id', 
+  inr ex, eff2 |
+IHB : ∀ σ : NameSub, ⟨ [], erase_names σ env (nth i exps ErrorExp) ⟩ -->* erase_result σ (inr ex)
+σ : NameSub
+______________________________________(1/1)
+⟨ [], erase_names σ env (EMap l) ⟩ -->* erase_result σ (inr ex)
+
+
+
+*)
+
+
+
+End tmp.
+
+
+
+
+
+
+
+
+
+
+
+
+(*
+////////////////////////////////////////////////////////////////////////////////
+//// EQBSFS_COMPOUNDS //////////////////////////////////////////////////////////
+////////////////////////////////////////////////////////////////////////////////
+*)
+
+Section tmp.
+
+(*
+
+env : Environment
+modules : list ErlModule
+own_module : string
+res : ValueSequence + Exception
+params : list Expression
+vals : list Value
+fname : string
+eff1, eff2 : SideEffectList
+eff : list SideEffectList
+ids : list nat
+id, id' : nat
+H : base.length params = base.length vals
+H0 : base.length params = base.length eff
+H1 : base.length params = base.length ids
+H2 :
+  ∀ i : nat,
+    i < base.length params
+    → | env, modules, own_module, nth_def ids id 0 i, nth i params ErrorExp, 
+      nth_def eff eff1 [] i | -e> | nth_def ids id 0 (S i), inl [nth i vals ErrorValue],
+      nth_def eff eff1 [] (S i) |
+H3 :
+  ∀ i : nat,
+    i < base.length params
+    → ∀ σ : NameSub,
+        ⟨ [], erase_names σ env (nth i params ErrorExp) ⟩ -->*
+        erase_result σ (inl [nth i vals ErrorValue])
+H4 : primop_eval fname vals (last eff eff1) = (res, eff2)
+H5 : id' = last ids id
+σ : NameSub
+______________________________________(1/1)
+⟨ [], erase_names σ env (EPrimOp fname params) ⟩ -->* erase_result σ res
+
+
+
+
+
+env : Environment
+modules : list ErlModule
+own_module : string
+i : nat
+fname : string
+params : list Expression
+vals : list Value
+ex : Exception
+eff1, eff2 : SideEffectList
+eff : list SideEffectList
+id, id' : nat
+ids : list nat
+H : i < base.length params
+H0 : base.length vals = i
+H1 : base.length eff = i
+H2 : base.length ids = i
+H3 :
+  ∀ j : nat,
+    j < i
+    → | env, modules, own_module, nth_def ids id 0 j, nth j params ErrorExp, 
+      nth_def eff eff1 [] j | -e> | nth_def ids id 0 (S j), inl [nth j vals ErrorValue],
+      nth_def eff eff1 [] (S j) |
+H4 :
+  ∀ j : nat,
+    j < i
+    → ∀ σ : NameSub,
+        ⟨ [], erase_names σ env (nth j params ErrorExp) ⟩ -->*
+        erase_result σ (inl [nth j vals ErrorValue])
+B :
+  | env, modules, own_module, last ids id, nth i params ErrorExp, last eff eff1 | -e> | id', 
+  inr ex, eff2 |
+IHB : ∀ σ : NameSub, ⟨ [], erase_names σ env (nth i params ErrorExp) ⟩ -->* erase_result σ (inr ex)
+σ : NameSub
+______________________________________(1/1)
+⟨ [], erase_names σ env (EPrimOp fname params) ⟩ -->* erase_result σ (inr ex)
+
+*)
+
+
+
+End tmp.
+
+Section tmp.
+
+(*
+
+params : list Expression
+vals : list Value
+env : Environment
+modules : list ErlModule
+own_module : string
+exp, body : Expression
+res : ValueSequence + Exception
+var_list : list Var
+ref : Environment
+ext : list (nat * FunctionIdentifier * FunctionExpression)
+n : nat
+eff1, eff2, eff3 : SideEffectList
+eff : list SideEffectList
+ids : list nat
+id, id', id'' : nat
+H : base.length params = base.length vals
+B1 :
+  | env, modules, own_module, id, exp, eff1 | -e> | id', inl [VClos ref ext n var_list body], eff2 |
+H0 : base.length var_list = base.length vals
+H1 : base.length params = base.length eff
+H2 : base.length params = base.length ids
+H3 :
+  ∀ i : nat,
+    i < base.length params
+    → | env, modules, own_module, nth_def ids id' 0 i, nth i params ErrorExp, 
+      nth_def eff eff2 [] i | -e> | nth_def ids id' 0 (S i), inl [nth i vals ErrorValue],
+      nth_def eff eff2 [] (S i) |
+H4 :
+  ∀ i : nat,
+    i < base.length params
+    → ∀ σ : NameSub,
+        ⟨ [], erase_names σ env (nth i params ErrorExp) ⟩ -->*
+        erase_result σ (inl [nth i vals ErrorValue])
+B2 :
+  | append_vars_to_env var_list vals (get_env ref ext), modules, own_module, 
+  last ids id', body, last eff eff2 | -e> | id'', res, eff3 |
+IHB1 :
+  ∀ σ : NameSub,
+    ⟨ [], erase_names σ env exp ⟩ -->* erase_result σ (inl [VClos ref ext n var_list body])
+IHB2 :
+  ∀ σ : NameSub,
+    ⟨ [], erase_names σ (append_vars_to_env var_list vals (get_env ref ext)) body ⟩ -->*
+    erase_result σ res
+σ : NameSub
+______________________________________(1/1)
+⟨ [], erase_names σ env (EApp exp params) ⟩ -->* erase_result σ res
+
+
+
+params : list Expression
+env : Environment
+modules : list ErlModule
+own_module : string
+exp : Expression
+ex : Exception
+eff1, eff2 : SideEffectList
+id, id' : nat
+B : | env, modules, own_module, id, exp, eff1 | -e> | id', inr ex, eff2 |
+IHB : ∀ σ : NameSub, ⟨ [], erase_names σ env exp ⟩ -->* erase_result σ (inr ex)
+σ : NameSub
+______________________________________(1/1)
+⟨ [], erase_names σ env (EApp exp params) ⟩ -->* erase_result σ (inr ex)
+
+
+
+params : list Expression
+vals : list Value
+env : Environment
+modules : list ErlModule
+own_module : string
+exp : Expression
+ex : Exception
+i : nat
+v : Value
+eff1, eff2, eff3 : SideEffectList
+eff : list SideEffectList
+ids : list nat
+id, id', id'' : nat
+H : i < base.length params
+H0 : base.length vals = i
+H1 : base.length eff = i
+H2 : base.length ids = i
+B1 : | env, modules, own_module, id, exp, eff1 | -e> | id', inl [v], eff2 |
+H3 :
+  ∀ j : nat,
+    j < i
+    → | env, modules, own_module, nth_def ids id' 0 j, nth j params ErrorExp, 
+      nth_def eff eff2 [] j | -e> | nth_def ids id' 0 (S j), inl [nth j vals ErrorValue],
+      nth_def eff eff2 [] (S j) |
+H4 :
+  ∀ j : nat,
+    j < i
+    → ∀ σ : NameSub,
+        ⟨ [], erase_names σ env (nth j params ErrorExp) ⟩ -->*
+        erase_result σ (inl [nth j vals ErrorValue])
+B2 :
+  | env, modules, own_module, last ids id', nth i params ErrorExp, last eff eff2 | -e> | id'',
+  inr ex, eff3 |
+IHB1 : ∀ σ : NameSub, ⟨ [], erase_names σ env exp ⟩ -->* erase_result σ (inl [v])
+IHB2 : ∀ σ : NameSub, ⟨ [], erase_names σ env (nth i params ErrorExp) ⟩ -->* erase_result σ (inr ex)
+σ : NameSub
+______________________________________(1/1)
+⟨ [], erase_names σ env (EApp exp params) ⟩ -->* erase_result σ (inr ex)
+
+
+
+
+params : list Expression
+vals : list Value
+env : Environment
+modules : list ErlModule
+own_module : string
+v : Value
+exp : Expression
+eff1, eff2, eff3 : SideEffectList
+eff : list SideEffectList
+ids : list nat
+id, id', id'' : nat
+H : base.length params = base.length vals
+H0 : base.length params = base.length eff
+H1 : base.length params = base.length ids
+B : | env, modules, own_module, id, exp, eff1 | -e> | id', inl [v], eff2 |
+H2 :
+  ∀ j : nat,
+    j < base.length params
+    → | env, modules, own_module, nth_def ids id' 0 j, nth j params ErrorExp, 
+      nth_def eff eff2 [] j | -e> | nth_def ids id' 0 (S j), inl [nth j vals ErrorValue],
+      nth_def eff eff2 [] (S j) |
+H3 :
+  ∀ j : nat,
+    j < base.length params
+    → ∀ σ : NameSub,
+        ⟨ [], erase_names σ env (nth j params ErrorExp) ⟩ -->*
+        erase_result σ (inl [nth j vals ErrorValue])
+H4 :
+  ∀ (ref : list ((Var + FunctionIdentifier) * Value)) (ext : list
+                                                               (nat * FunctionIdentifier *
+                                                                FunctionExpression)) 
+    (var_list : list Var) (body : Expression) (n : nat), v ≠ VClos ref ext n var_list body
+H5 : eff3 = last eff eff2
+H6 : id'' = last ids id'
+IHB : ∀ σ : NameSub, ⟨ [], erase_names σ env exp ⟩ -->* erase_result σ (inl [v])
+σ : NameSub
+______________________________________(1/1)
+⟨ [], erase_names σ env (EApp exp params) ⟩ -->* erase_result σ (inr (badfun v))
+
+
+
+
+
+params : list Expression
+vals : list Value
+env : Environment
+modules : list ErlModule
+own_module : string
+exp, body : Expression
+var_list : list Var
+ref : Environment
+ext : list (nat * FunctionIdentifier * FunctionExpression)
+eff1, eff2, eff3 : SideEffectList
+eff : list SideEffectList
+n : nat
+ids : list nat
+id, id', id'' : nat
+H : base.length params = base.length vals
+H0 : base.length params = base.length eff
+H1 : base.length params = base.length ids
+B :
+  | env, modules, own_module, id, exp, eff1 | -e> | id', inl [VClos ref ext n var_list body], eff2 |
+H2 :
+  ∀ j : nat,
+    j < base.length params
+    → | env, modules, own_module, nth_def ids id' 0 j, nth j params ErrorExp, 
+      nth_def eff eff2 [] j | -e> | nth_def ids id' 0 (S j), inl [nth j vals ErrorValue],
+      nth_def eff eff2 [] (S j) |
+H3 :
+  ∀ j : nat,
+    j < base.length params
+    → ∀ σ : NameSub,
+        ⟨ [], erase_names σ env (nth j params ErrorExp) ⟩ -->*
+        erase_result σ (inl [nth j vals ErrorValue])
+H4 : base.length var_list ≠ base.length vals
+H5 : eff3 = last eff eff2
+H6 : id'' = last ids id'
+IHB :
+  ∀ σ : NameSub,
+    ⟨ [], erase_names σ env exp ⟩ -->* erase_result σ (inl [VClos ref ext n var_list body])
+σ : NameSub
+______________________________________(1/1)
+⟨ [], erase_names σ env (EApp exp params) ⟩ -->*
+erase_result σ (inr (badarity (VClos ref ext n var_list body)))
+
+
+
+
+
+*)
+
+
+
+End tmp.
+
+Section tmp.
+
+(*
+
+env : Environment
+modules : list ErlModule
+own_module : string
+res : ValueSequence + Exception
+params : list Expression
+vals : list Value
+mexp, fexp : Expression
+mname, fname : string
+eff1, eff2, eff3, eff4 : SideEffectList
+eff : list SideEffectList
+ids : list nat
+id, id', id'', id''' : nat
+H : base.length params = base.length vals
+H0 : base.length params = base.length eff
+H1 : base.length params = base.length ids
+B1 : | env, modules, own_module, id, mexp, eff1 | -e> | id', inl [VLit (Atom mname)], eff2 |
+B2 : | env, modules, own_module, id', fexp, eff2 | -e> | id'', inl [VLit (Atom fname)], eff3 |
+H2 :
+  ∀ i : nat,
+    i < base.length params
+    → | env, modules, own_module, nth_def ids id'' 0 i, nth i params ErrorExp, 
+      nth_def eff eff3 [] i | -e> | nth_def ids id'' 0 (S i), inl [nth i vals ErrorValue],
+      nth_def eff eff3 [] (S i) |
+H3 :
+  ∀ i : nat,
+    i < base.length params
+    → ∀ σ : NameSub,
+        ⟨ [], erase_names σ env (nth i params ErrorExp) ⟩ -->*
+        erase_result σ (inl [nth i vals ErrorValue])
+H4 : get_modfunc mname fname (base.length vals) (modules ++ stdlib) = None
+H5 : eval mname fname vals (last eff eff3) = (res, eff4)
+H6 : id''' = last ids id''
+IHB1 : ∀ σ : NameSub, ⟨ [], erase_names σ env mexp ⟩ -->* erase_result σ (inl [VLit (Atom mname)])
+IHB2 : ∀ σ : NameSub, ⟨ [], erase_names σ env fexp ⟩ -->* erase_result σ (inl [VLit (Atom fname)])
+σ : NameSub
+______________________________________(1/1)
+⟨ [], erase_names σ env (ECall mexp fexp params) ⟩ -->* erase_result σ res
+
+
+
+
+
+env : Environment
+modules : list ErlModule
+own_module : string
+res : ValueSequence + Exception
+params : list Expression
+vals : list Value
+mexp, fexp : Expression
+mname, fname : string
+func : TopLevelFunction
+eff1, eff2, eff3, eff4 : SideEffectList
+eff : list SideEffectList
+ids : list nat
+id, id', id'', id''' : nat
+H : base.length params = base.length vals
+H0 : base.length params = base.length eff
+H1 : base.length params = base.length ids
+B1 : | env, modules, own_module, id, mexp, eff1 | -e> | id', inl [VLit (Atom mname)], eff2 |
+B2 : | env, modules, own_module, id', fexp, eff2 | -e> | id'', inl [VLit (Atom fname)], eff3 |
+H2 :
+  ∀ i : nat,
+    i < base.length params
+    → | env, modules, own_module, nth_def ids id'' 0 i, nth i params ErrorExp, 
+      nth_def eff eff3 [] i | -e> | nth_def ids id'' 0 (S i), inl [nth i vals ErrorValue],
+      nth_def eff eff3 [] (S i) |
+H3 :
+  ∀ i : nat,
+    i < base.length params
+    → ∀ σ : NameSub,
+        ⟨ [], erase_names σ env (nth i params ErrorExp) ⟩ -->*
+        erase_result σ (inl [nth i vals ErrorValue])
+H4 : get_modfunc mname fname (base.length vals) (modules ++ stdlib) = Some func
+B3 :
+  | append_vars_to_env (varl func) vals [], modules, mname, last ids id'', 
+  body func, last eff eff3 | -e> | id''', res, eff4 |
+IHB1 : ∀ σ : NameSub, ⟨ [], erase_names σ env mexp ⟩ -->* erase_result σ (inl [VLit (Atom mname)])
+IHB2 : ∀ σ : NameSub, ⟨ [], erase_names σ env fexp ⟩ -->* erase_result σ (inl [VLit (Atom fname)])
+IHB3 :
+  ∀ σ : NameSub,
+    ⟨ [], erase_names σ (append_vars_to_env (varl func) vals []) (body func) ⟩ -->*
+    erase_result σ res
+σ : NameSub
+______________________________________(1/1)
+⟨ [], erase_names σ env (ECall mexp fexp params) ⟩ -->* erase_result σ res
+
+
+
+
+
+
+
+env : Environment
+modules : list ErlModule
+own_module : string
+i : nat
+mexp, fexp : Expression
+v, v' : Value
+params : list Expression
+vals : list Value
+ex : Exception
+eff1, eff2, eff3, eff4 : SideEffectList
+eff : list SideEffectList
+id, id', id'', id''' : nat
+ids : list nat
+H : i < base.length params
+H0 : base.length vals = i
+H1 : base.length eff = i
+H2 : base.length ids = i
+B1 : | env, modules, own_module, id, mexp, eff1 | -e> | id', inl [v], eff2 |
+B2 : | env, modules, own_module, id', fexp, eff2 | -e> | id'', inl [v'], eff3 |
+H3 :
+  ∀ j : nat,
+    j < i
+    → | env, modules, own_module, nth_def ids id'' 0 j, nth j params ErrorExp, 
+      nth_def eff eff3 [] j | -e> | nth_def ids id'' 0 (S j), inl [nth j vals ErrorValue],
+      nth_def eff eff3 [] (S j) |
+H4 :
+  ∀ j : nat,
+    j < i
+    → ∀ σ : NameSub,
+        ⟨ [], erase_names σ env (nth j params ErrorExp) ⟩ -->*
+        erase_result σ (inl [nth j vals ErrorValue])
+B3 :
+  | env, modules, own_module, last ids id'', nth i params ErrorExp, last eff eff3 | -e> | id''',
+  inr ex, eff4 |
+IHB1 : ∀ σ : NameSub, ⟨ [], erase_names σ env mexp ⟩ -->* erase_result σ (inl [v])
+IHB2 : ∀ σ : NameSub, ⟨ [], erase_names σ env fexp ⟩ -->* erase_result σ (inl [v'])
+IHB3 : ∀ σ : NameSub, ⟨ [], erase_names σ env (nth i params ErrorExp) ⟩ -->* erase_result σ (inr ex)
+σ : NameSub
+______________________________________(1/1)
+⟨ [], erase_names σ env (ECall mexp fexp params) ⟩ -->* erase_result σ (inr ex)
+
+
+
+
+
+
+
+env : Environment
+modules : list ErlModule
+own_module : string
+mexp, fexp : Expression
+params : list Expression
+ex : Exception
+eff1, eff2 : SideEffectList
+id, id' : nat
+B : | env, modules, own_module, id, mexp, eff1 | -e> | id', inr ex, eff2 |
+IHB : ∀ σ : NameSub, ⟨ [], erase_names σ env mexp ⟩ -->* erase_result σ (inr ex)
+σ : NameSub
+______________________________________(1/1)
+⟨ [], erase_names σ env (ECall mexp fexp params) ⟩ -->* erase_result σ (inr ex)
+
+
+
+
+
+
+env : Environment
+modules : list ErlModule
+own_module : string
+mexp, fexp : Expression
+v : Value
+params : list Expression
+ex : Exception
+eff1, eff2, eff3 : SideEffectList
+id, id', id'' : nat
+B1 : | env, modules, own_module, id, mexp, eff1 | -e> | id', inl [v], eff2 |
+B2 : | env, modules, own_module, id', fexp, eff2 | -e> | id'', inr ex, eff3 |
+IHB1 : ∀ σ : NameSub, ⟨ [], erase_names σ env mexp ⟩ -->* erase_result σ (inl [v])
+IHB2 : ∀ σ : NameSub, ⟨ [], erase_names σ env fexp ⟩ -->* erase_result σ (inr ex)
+σ : NameSub
+______________________________________(1/1)
+⟨ [], erase_names σ env (ECall mexp fexp params) ⟩ -->* erase_result σ (inr ex)
+
+
+
+
+
+env : Environment
+modules : list ErlModule
+own_module : string
+mexp, fexp : Expression
+v, v' : Value
+params : list Expression
+vals : list Value
+eff1, eff2, eff3, eff4 : SideEffectList
+eff : list SideEffectList
+id, id', id'', id''' : nat
+ids : list nat
+H : base.length params = base.length vals
+H0 : base.length params = base.length eff
+H1 : base.length params = base.length ids
+B1 : | env, modules, own_module, id, mexp, eff1 | -e> | id', inl [v], eff2 |
+B2 : | env, modules, own_module, id', fexp, eff2 | -e> | id'', inl [v'], eff3 |
+H2 :
+  ∀ i : nat,
+    i < base.length params
+    → | env, modules, own_module, nth_def ids id'' 0 i, nth i params ErrorExp, 
+      nth_def eff eff3 [] i | -e> | nth_def ids id'' 0 (S i), inl [nth i vals ErrorValue],
+      nth_def eff eff3 [] (S i) |
+H3 :
+  ∀ i : nat,
+    i < base.length params
+    → ∀ σ : NameSub,
+        ⟨ [], erase_names σ env (nth i params ErrorExp) ⟩ -->*
+        erase_result σ (inl [nth i vals ErrorValue])
+H4 : ∀ mname : string, v ≠ VLit (Atom mname)
+H5 : eff4 = last eff eff3
+H6 : id''' = last ids id''
+IHB1 : ∀ σ : NameSub, ⟨ [], erase_names σ env mexp ⟩ -->* erase_result σ (inl [v])
+IHB2 : ∀ σ : NameSub, ⟨ [], erase_names σ env fexp ⟩ -->* erase_result σ (inl [v'])
+σ : NameSub
+______________________________________(1/1)
+⟨ [], erase_names σ env (ECall mexp fexp params) ⟩ -->* erase_result σ (inr (badarg v))
+
+
+
+
+
+
+
+env : Environment
+modules : list ErlModule
+own_module : string
+mexp, fexp : Expression
+mname : string
+v' : Value
+params : list Expression
+vals : list Value
+eff1, eff2, eff3, eff4 : SideEffectList
+eff : list SideEffectList
+id, id', id'', id''' : nat
+ids : list nat
+H : base.length params = base.length vals
+H0 : base.length params = base.length eff
+H1 : base.length params = base.length ids
+B1 : | env, modules, own_module, id, mexp, eff1 | -e> | id', inl [VLit (Atom mname)], eff2 |
+B2 : | env, modules, own_module, id', fexp, eff2 | -e> | id'', inl [v'], eff3 |
+H2 :
+  ∀ i : nat,
+    i < base.length params
+    → | env, modules, own_module, nth_def ids id'' 0 i, nth i params ErrorExp, 
+      nth_def eff eff3 [] i | -e> | nth_def ids id'' 0 (S i), inl [nth i vals ErrorValue],
+      nth_def eff eff3 [] (S i) |
+H3 :
+  ∀ i : nat,
+    i < base.length params
+    → ∀ σ : NameSub,
+        ⟨ [], erase_names σ env (nth i params ErrorExp) ⟩ -->*
+        erase_result σ (inl [nth i vals ErrorValue])
+H4 : ∀ fname : string, v' ≠ VLit (Atom fname)
+H5 : eff4 = last eff eff3
+H6 : id''' = last ids id''
+IHB1 : ∀ σ : NameSub, ⟨ [], erase_names σ env mexp ⟩ -->* erase_result σ (inl [VLit (Atom mname)])
+IHB2 : ∀ σ : NameSub, ⟨ [], erase_names σ env fexp ⟩ -->* erase_result σ (inl [v'])
+σ : NameSub
+______________________________________(1/1)
+⟨ [], erase_names σ env (ECall mexp fexp params) ⟩ -->* erase_result σ (inr (badarg v'))
+
+
+*)
+
+
+
+End tmp.
+
+Section tmp.
+
+(*
+
+env : Environment
+modules : list ErlModule
+own_module : string
+guard, exp, e : Expression
+vals : ValueSequence
+res : ValueSequence + Exception
+l : list (list Pattern * Expression * Expression)
+bindings : list (Var * Value)
+i : nat
+eff1, eff2, eff3 : SideEffectList
+id, id', id'' : nat
+B1 : | env, modules, own_module, id, e, eff1 | -e> | id', inl vals, eff2 |
+H : i < base.length l
+H0 : match_clause vals l i = Some (guard, exp, bindings)
+H1 :
+  ∀ j : nat,
+    j < i
+    → ∀ (gg ee : Expression) (bb : list (Var * Value)),
+        match_clause vals l j = Some (gg, ee, bb)
+        → | add_bindings bb env, modules, own_module, id', gg, eff2 | -e> | id', 
+          inl [ffalse], eff2 |
+H2 :
+  ∀ j : nat,
+    j < i
+    → ∀ (gg ee : Expression) (bb : list (Var * Value)),
+        match_clause vals l j = Some (gg, ee, bb)
+        → ∀ σ : NameSub,
+            ⟨ [], erase_names σ (add_bindings bb env) gg ⟩ -->* erase_result σ (inl [ffalse])
+B2 :
+  | add_bindings bindings env, modules, own_module, id', guard, eff2 | -e> | id', 
+  inl [ttrue], eff2 |
+B3 : | add_bindings bindings env, modules, own_module, id', exp, eff2 | -e> | id'', res, eff3 |
+IHB1 : ∀ σ : NameSub, ⟨ [], erase_names σ env e ⟩ -->* erase_result σ (inl vals)
+IHB2 :
+  ∀ σ : NameSub,
+    ⟨ [], erase_names σ (add_bindings bindings env) guard ⟩ -->* erase_result σ (inl [ttrue])
+IHB3 : ∀ σ : NameSub, ⟨ [], erase_names σ (add_bindings bindings env) exp ⟩ -->* erase_result σ res
+σ : NameSub
+______________________________________(1/1)
+⟨ [], erase_names σ env (ECase e l) ⟩ -->* erase_result σ res
+
+
+
+
+env : Environment
+modules : list ErlModule
+own_module : string
+e : Expression
+ex : Exception
+l : list (list Pattern * Expression * Expression)
+eff1, eff2 : SideEffectList
+id, id' : nat
+B : | env, modules, own_module, id, e, eff1 | -e> | id', inr ex, eff2 |
+IHB : ∀ σ : NameSub, ⟨ [], erase_names σ env e ⟩ -->* erase_result σ (inr ex)
+σ : NameSub
+______________________________________(1/1)
+⟨ [], erase_names σ env (ECase e l) ⟩ -->* erase_result σ (inr ex)
+
+
+
+
+env : Environment
+modules : list ErlModule
+own_module : string
+e : Expression
+l : list (list Pattern * Expression * Expression)
+vals : ValueSequence
+eff1, eff2 : SideEffectList
+id, id' : nat
+B : | env, modules, own_module, id, e, eff1 | -e> | id', inl vals, eff2 |
+H :
+  ∀ j : nat,
+    j < base.length l
+    → ∀ (gg ee : Expression) (bb : list (Var * Value)),
+        match_clause vals l j = Some (gg, ee, bb)
+        → | add_bindings bb env, modules, own_module, id', gg, eff2 | -e> | id', 
+          inl [ffalse], eff2 |
+H0 :
+  ∀ j : nat,
+    j < base.length l
+    → ∀ (gg ee : Expression) (bb : list (Var * Value)),
+        match_clause vals l j = Some (gg, ee, bb)
+        → ∀ σ : NameSub,
+            ⟨ [], erase_names σ (add_bindings bb env) gg ⟩ -->* erase_result σ (inl [ffalse])
+IHB : ∀ σ : NameSub, ⟨ [], erase_names σ env e ⟩ -->* erase_result σ (inl vals)
+σ : NameSub
+______________________________________(1/1)
+⟨ [], erase_names σ env (ECase e l) ⟩ -->* erase_result σ (inr if_clause)
+
+
+
+env : Environment
+modules : list ErlModule
+own_module : string
+e, guard, exp : Expression
+bindings : list (Var * Value)
+l : list (list Pattern * Expression * Expression)
+i : nat
+vals : ValueSequence
+ex : Exception
+eff1, eff2 : SideEffectList
+id, id' : nat
+B1 : | env, modules, own_module, id, e, eff1 | -e> | id', inl vals, eff2 |
+H : i < base.length l
+H0 : match_clause vals l i = Some (guard, exp, bindings)
+H1 :
+  ∀ j : nat,
+    j < i
+    → ∀ (gg ee : Expression) (bb : list (Var * Value)),
+        match_clause vals l j = Some (gg, ee, bb)
+        → | add_bindings bb env, modules, own_module, id', gg, eff2 | -e> | id', 
+          inl [ffalse], eff2 |
+H2 :
+  ∀ j : nat,
+    j < i
+    → ∀ (gg ee : Expression) (bb : list (Var * Value)),
+        match_clause vals l j = Some (gg, ee, bb)
+        → ∀ σ : NameSub,
+            ⟨ [], erase_names σ (add_bindings bb env) gg ⟩ -->* erase_result σ (inl [ffalse])
+B2 : | add_bindings bindings env, modules, own_module, id', guard, eff2 | -e> | id', inr ex, eff2 |
+IHB1 : ∀ σ : NameSub, ⟨ [], erase_names σ env e ⟩ -->* erase_result σ (inl vals)
+IHB2 :
+  ∀ σ : NameSub,
+    ⟨ [], erase_names σ (add_bindings bindings env) guard ⟩ -->* erase_result σ (inr ex)
+σ : NameSub
+______________________________________(1/1)
+⟨ [], erase_names σ env (ECase e l) ⟩ -->* erase_result σ (inr ex)
+
+
+
+*)
+
+
+
+
+
+
+End tmp.
+
+
+
+
+
+
+
+
+
+
+
+
+(*
+////////////////////////////////////////////////////////////////////////////////
+//// EQBSFS_MAIN ///////////////////////////////////////////////////////////////
+////////////////////////////////////////////////////////////////////////////////
+*)
+
+Section tmp.
+
+
+
+End tmp.
+
+
