src/Eqvivalence/BsFs/Helpers.v
@@ -1,0 +1,1038 @@
+From CoreErlang.Eqvivalence.BsFs Require Export EraseNames.
+
+Import SubstSemantics.
+
+(** CONTENT:
+* SCOPE (LEMMAS & TACTICS)
+  - Scope_Destructs (TACTICS)
+    + des_for
+  - Scope_Lists (LEMMAS)
+    + scope_list_succ
+    + scope_list_succ_id
+  - Scope_Values (THEOREMS)
+    + scope_vcons
+    + scope_vtuple
+    + scope_vmap
+  - Scope_Tactics (TACTICS)
+    + scope
+    + start
+* STEP (TACTICS)
+  - Step
+    + do_step
+    + do_transitive
+    + step
+* ENVIRONMENT_LEMMAS (LEMMAS)
+  - EnvironmentLemmas_GetValue
+    + get_value_singleton
+    + get_value_singleton_length
+    + get_value_single_det
+    + get_value_cons
+  - EnvironmentLemmas_Remove
+* ERASER_SUBST_APPEND (LEMMAS & THEOREMS)
+  - EraserSubstAppend_EraserLemmas (LEMMAS)
+    + add_keys_app
+    + add_keys_get_env_app
+    + add_keys_append_vars_to_env_app
+    + add_keys_append_vars_to_env_get_env_app
+    + add_keys_append_funs_to_env_app
+  - EraserSubstAppend_SubstLemmas (LEMMAS)
+    + list_subst_cons
+    + list_subst_fold_right
+    + list_subst_app
+  - EraserSubstAppend_Theorems (THEOREMS)
+    + erase_exp_append_vars
+* FRAMEIDENT (LEMMAS)
+  * BIFORALL ?
+  * CREATE_RESULTS
+* AXIOMS
+
+*)
+
+
+
+
+
+
+
+
+
+
+
+
+(*
+////////////////////////////////////////////////////////////////////////////////
+//// CHAPTER: SCOPE ////////////////////////////////////////////////////////////
+////////////////////////////////////////////////////////////////////////////////
+*)
+
+
+
+
+
+
+(* Section Scope_Destructs. *)
+
+
+
+  (** DOCUMENTATION:
+  * des_for --> destruct_foralls; rename
+    - N:[ident]:1-10 : N:[ident]:1-10
+  *)
+
+  Tactic Notation "des_for"
+      :=
+    destruct_foralls.
+
+  Tactic Notation "des_for"
+      "-"   ident(In1)
+      ":"   ident(Io1)
+      :=
+    destruct_foralls;
+    ren - In1:
+          Io1.
+
+  Tactic Notation "des_for"
+      "-"   ident(In1) ident(In2)
+      ":"   ident(Io1) ident(Io2)
+      :=
+    destruct_foralls;
+    ren - In1 In2:
+          Io1 Io2.
+
+  Tactic Notation "des_for"
+      "-"   ident(In1) ident(In2) ident(In3)
+      ":"   ident(Io1) ident(Io2) ident(Io3)
+      :=
+    destruct_foralls;
+    ren - In1 In2 In3:
+          Io1 Io2 Io3.
+
+  Tactic Notation "des_for"
+      "-"   ident(In1) ident(In2) ident(In3) ident(In4)
+      ":"   ident(Io1) ident(Io2) ident(Io3) ident(Io4)
+      :=
+    destruct_foralls;
+    ren - In1 In2 In3 In4:
+          Io1 Io2 Io3 Io4.
+
+  Tactic Notation "des_for"
+      "-"   ident(In1) ident(In2) ident(In3) ident(In4) ident(In5)
+      ":"   ident(Io1) ident(Io2) ident(Io3) ident(Io4) ident(Io5)
+      :=
+    destruct_foralls;
+    ren - In1 In2 In3 In4 In5:
+          Io1 Io2 Io3 Io4 Io5.
+
+  Tactic Notation "des_for"
+      "-"   ident(In1) ident(In2) ident(In3) ident(In4) ident(In5)
+            ident(In6)
+      ":"   ident(Io1) ident(Io2) ident(Io3) ident(Io4) ident(Io5)
+            ident(Io6)
+      :=
+    destruct_foralls;
+    ren - In1 In2 In3 In4 In5 In6:
+          Io1 Io2 Io3 Io4 Io5 Io6.
+
+  Tactic Notation "des_for"
+      "-"   ident(In1) ident(In2) ident(In3) ident(In4) ident(In5)
+            ident(In6) ident(In7)
+      ":"   ident(Io1) ident(Io2) ident(Io3) ident(Io4) ident(Io5)
+            ident(Io6) ident(Io7)
+      :=
+    destruct_foralls;
+    ren - In1 In2 In3 In4 In5 In6 In7:
+          Io1 Io2 Io3 Io4 Io5 Io6 Io7.
+
+  Tactic Notation "des_for"
+      "-"   ident(In1) ident(In2) ident(In3) ident(In4) ident(In5)
+            ident(In6) ident(In7) ident(In8)
+      ":"   ident(Io1) ident(Io2) ident(Io3) ident(Io4) ident(Io5)
+            ident(Io6) ident(Io7) ident(Io8)
+      :=
+    destruct_foralls;
+    ren - In1 In2 In3 In4 In5 In6 In7 In8:
+          Io1 Io2 Io3 Io4 Io5 Io6 Io7 Io8.
+
+  Tactic Notation "des_for"
+      "-"   ident(In1) ident(In2) ident(In3) ident(In4) ident(In5)
+            ident(In6) ident(In7) ident(In8) ident(In9)
+      ":"   ident(Io1) ident(Io2) ident(Io3) ident(Io4) ident(Io5)
+            ident(Io6) ident(Io7) ident(Io8) ident(Io9)
+      :=
+    destruct_foralls;
+    ren - In1 In2 In3 In4 In5 In6 In7 In8 In9:
+          Io1 Io2 Io3 Io4 Io5 Io6 Io7 Io8 Io9.
+
+  Tactic Notation "des_for"
+      "-"   ident(In1) ident(In2) ident(In3) ident(In4) ident(In5)
+            ident(In6) ident(In7) ident(In8) ident(In9) ident(In10)
+      ":"   ident(Io1) ident(Io2) ident(Io3) ident(Io4) ident(Io5)
+            ident(Io6) ident(Io7) ident(Io8) ident(Io9) ident(Io10)
+      :=
+    destruct_foralls;
+    ren - In1 In2 In3 In4 In5 In6 In7 In8 In9 In10:
+          Io1 Io2 Io3 Io4 Io5 Io6 Io7 Io8 Io9 Io10.
+
+
+
+(* End Scope_Destructs. *)
+
+
+
+
+
+
+
+
+
+Section Scope_Lists.
+
+
+
+  Lemma scope_list_succ :
+    forall A i vl (f : A -> Val),
+        (i < length vl
+        ->  VALCLOSED (nth i (map f vl) VNil))
+    ->  (S i < S (length vl)
+        ->  VALCLOSED (nth i (map f vl) VNil)).
+  Proof.
+    (* #1 Pose: intro/pose/destruct/ *)
+    itr - A i vl f Hvl Hsucc_lt.
+    pse - Nat.succ_lt_mono as Hmono_succ_lt: i (base.length vl).
+    des - Hmono_succ_lt as [_ Hfrom_succ_lt].
+    (* #2 Apply: apply *)
+    app - Hfrom_succ_lt in Hsucc_lt as Hlt; clr - Hfrom_succ_lt.
+    bpp - Hvl in Hlt.
+  Qed.
+
+
+
+  Lemma scope_list_succ_id :
+    forall i vl,
+        (i < length vl
+        ->  VALCLOSED (nth i vl VNil))
+    ->  (S i < S (length vl)
+        ->  VALCLOSED (nth i vl VNil)).
+  Proof.
+    (* #1 Assert: intro/assert/remember + apply *)
+    itr - i vl Hvl.
+    ass > (map id vl = vl) as Hid: apply Basics.map_id.
+    rem - n as Hn: (base.length vl).
+    (* #2 Rewrite: rewrite *)
+    cwl + Hid in Hvl.
+    cwr - Hn in *.
+    (* #3 Pose by Previus: pose *)
+    by pose proof scope_list_succ Val i vl id Hvl.
+  Qed.
+
+
+
+End Scope_Lists.
+
+
+
+
+
+
+
+
+
+Section Scope_Value.
+
+
+
+  Theorem scope_vcons :
+    forall v1 v2,
+        is_result (RValSeq [v1])
+    ->  is_result (RValSeq [v2])
+    ->  is_result (RValSeq [VCons v1 v2]).
+  Proof.
+    (* #1 Inversion: intro/inversion/destruct_foralls *)
+    itr - v1 v2 Hv1 Hv2.
+    ivc - Hv1 as Hv1: H0.
+    ivc - Hv2 as Hv2: H0.
+    des_for - Hv1 Hv2: H3 H1.
+    (* #2 Finish: pose *)
+    ato.
+  Qed.
+
+
+
+  Theorem scope_vtuple :
+    forall v vl,
+        is_result (RValSeq [v])
+    ->  is_result (RValSeq [VTuple vl])
+    ->  is_result (RValSeq [VTuple (v :: vl)]).
+  Proof.
+    (* #1 Inversion: intro/inversion/destruct_foralls *)
+    itr - v vl Hv Hvl.
+    ivc - Hv as Hv: H0.
+    ivc - Hvl as Hvl: H0.
+    des_for - Hv Hvl: H3 H1.
+    (* #3 Constructor: constructor *)
+    do 3 cns.
+    (* #4 Simplify: intro/simpl *)
+    itr - i Hl.
+    smp *.
+    (* #5 Destruct: destruct + exact *)
+    des - i: exa - Hv.
+    (* #6 Inversion: inversion *)
+    ivc - Hvl as Hvl: H1 / v Hv.
+    (* #7 Finish: pose *)
+    bse - scope_list_succ_id: i vl (Hvl i) Hl.
+  Qed.
+
+
+
+  Theorem scope_vmap :
+    forall v1 v2 vl,
+        is_result (RValSeq [v1])
+    ->  is_result (RValSeq [v2])
+    ->  is_result (RValSeq [VMap vl])
+    ->  is_result (RValSeq [VMap ((v1, v2) :: vl)]).
+  Proof.
+    (* #1 Inversion: intro/inversion/destruct_foralls *)
+    itr - v1 v2 vl Hv1 Hv2 Hvl.
+    ivc - Hv1 as Hv1: H0.
+    ivc - Hv2 as Hv2: H0.
+    ivc - Hvl as Hvl: H0.
+    des_for - Hv1 Hv2 Hvl: H5 H3 H1.
+    (* #3 Constructor: constructor *)
+    do 3 cns.
+    * (* #4.1 Simplify: intro/simpl *)
+      itr - i Hl.
+      smp *.
+      (* #5.1 Destruct: clear/destruct + exact *)
+      clr - Hv2 v2.
+      des - i: exa - Hv1.
+      (* #6.1 Inversion: inversion *)
+      ivc - Hvl as Hvl: H0 / H2 v1 Hv1.
+      (* #7.1 Finish: pose *)
+      by pose proof scope_list_succ (Val * Val) i vl fst (Hvl i) Hl.
+    * (* #4.2 Simplify: intro/simpl *)
+      itr - i Hl.
+      smp *.
+      (* #5.2 Destruct: clear/destruct + exact *)
+      clr - Hv1 v1.
+      des - i: exa - Hv2.
+      (* #6.2 Inversion: inversion *)
+      ivc - Hvl as Hvl: H2 / H0 v2 Hv2.
+      (* #7.2 Finish: pose *)
+      by pose proof scope_list_succ (Val * Val) i vl snd (Hvl i) Hl.
+  Qed.
+
+
+
+End Scope_Value.
+
+
+
+
+
+
+
+
+
+(* Section Scope_Tactics. *)
+
+
+
+  Ltac scope :=
+    try (apply scope_vcons; [assumption ..]);
+    try (apply scope_vtuple; [assumption ..]);
+    try (apply scope_vmap; [assumption ..]);
+    try (constructor);
+    try (destruct_foralls);
+    try (assumption + scope_solver).
+
+
+
+  (** DOCUMENTATION:
+  * start --> eexists; split; [> scope]; clear.
+    / [ident]:0-3
+    - hyp
+  *)
+
+  Tactic Notation "start"
+      :=
+    eexists; split; [(scope + admit) | idtac].
+
+  Tactic Notation "start"
+      "/"   ident(I1)
+      :=
+    eexists; split; [(scope + admit) | idtac];
+    clear I1.
+
+  Tactic Notation "start"
+      "/"   ident(I1) ident(I2)
+      :=
+    eexists; split; [(scope + admit) | idtac];
+    clear I1 I2.
+
+  Tactic Notation "start"
+      "/"   ident(I1) ident(I2) ident(I3)
+      :=
+    eexists; split; [(scope + admit) | idtac];
+    clear I1 I2 I3.
+
+  Tactic Notation "start"
+      "-"   ident(H)
+      :=
+    eexists; split; [ivs - H; (scope + admit) | clear H].
+
+
+
+(* End Scope_Tactics. *)
+
+
+
+
+
+
+
+
+
+
+
+
+(*
+////////////////////////////////////////////////////////////////////////////////
+//// CHAPTER: STEP /////////////////////////////////////////////////////////////
+////////////////////////////////////////////////////////////////////////////////
+*)
+
+
+
+
+
+
+(* Section Step. *)
+
+
+
+  Ltac do_step
+    :=
+    (econstructor;
+    [ (constructor; auto + scope_solver + congruence)
+    + (econstructor; constructor)
+    + (econstructor;
+      [ congruence
+      | constructor ])
+    | simpl ])
+    + (cbn; constructor).
+
+
+
+  Ltac do_transitive H
+    :=
+    eapply transitive_eval;
+    [ eapply frame_indep_core in H;
+      exact H
+    | clear H;
+      simpl ].
+
+
+
+  (** DOCUMENTATION:
+  * step --> repeat step; (exact H + do_transitive H).
+    - hyp / [ident]:0-10
+  *)
+
+  Tactic Notation "step"
+      :=
+    repeat do_step.
+
+  Tactic Notation "step"
+      "-"   hyp(H)
+      :=
+    repeat do_step;
+    (exact H + do_transitive H).
+
+  Tactic Notation "step"
+      "-"   hyp(H)
+      "/"   ident(I1)
+      :=
+    repeat do_step;
+    (exact H + do_transitive H);
+    clear I1.
+
+  Tactic Notation "step"
+      "-"   hyp(H)
+      "/"   ident(I1) ident(I2)
+      :=
+    repeat do_step;
+    (exact H + do_transitive H);
+    clear I1 I2.
+
+  Tactic Notation "step"
+      "-"   hyp(H)
+      "/"   ident(I1) ident(I2) ident(I3)
+      :=
+    repeat do_step;
+    (exact H + do_transitive H);
+    clear I1 I2 I3.
+
+  Tactic Notation "step"
+      "-"   hyp(H)
+      "/"   ident(I1) ident(I2) ident(I3) ident(I4)
+      :=
+    repeat do_step;
+    (exact H + do_transitive H);
+    clear I1 I2 I3 I4.
+
+  Tactic Notation "step"
+      "-"   hyp(H)
+      "/"   ident(I1) ident(I2) ident(I3) ident(I4) ident(I5)
+      :=
+    repeat do_step;
+    (exact H + do_transitive H);
+    clear I1 I2 I3 I4 I5.
+
+  Tactic Notation "step"
+      "-"   hyp(H)
+      "/"   ident(I1) ident(I2) ident(I3) ident(I4) ident(I5)
+            ident(I6)
+      :=
+    repeat do_step;
+    (exact H + do_transitive H);
+    clear I1 I2 I3 I4 I5 I6.
+
+  Tactic Notation "step"
+      "-"   hyp(H)
+      "/"   ident(I1) ident(I2) ident(I3) ident(I4) ident(I5)
+            ident(I6) ident(I7)
+      :=
+    repeat do_step;
+    (exact H + do_transitive H);
+    clear I1 I2 I3 I4 I5 I6 I7.
+
+  Tactic Notation "step"
+      "-"   hyp(H)
+      "/"   ident(I1) ident(I2) ident(I3) ident(I4) ident(I5)
+            ident(I6) ident(I7) ident(I8)
+      :=
+    repeat do_step;
+    (exact H + do_transitive H);
+    clear I1 I2 I3 I4 I5 I6 I7 I8.
+
+  Tactic Notation "step"
+      "-"   hyp(H)
+      "/"   ident(I1) ident(I2) ident(I3) ident(I4) ident(I5)
+            ident(I6) ident(I7) ident(I8) ident(I9)
+      :=
+    repeat do_step;
+    (exact H + do_transitive H);
+    clear I1 I2 I3 I4 I5 I6 I7 I8 I9.
+
+  Tactic Notation "step"
+      "-"   hyp(H)
+      "/"   ident(I1) ident(I2) ident(I3) ident(I4) ident(I5)
+            ident(I6) ident(I7) ident(I8) ident(I9) ident(I10)
+      :=
+    repeat do_step;
+    (exact H + do_transitive H);
+    clear I1 I2 I3 I4 I5 I6 I7 I8 I9 I10.
+
+
+
+(* End Step. *)
+
+
+
+
+
+
+
+
+
+
+
+
+(*
+////////////////////////////////////////////////////////////////////////////////
+//// CHAPTER: ENVIRONMENT_LEMMAS ///////////////////////////////////////////////
+////////////////////////////////////////////////////////////////////////////////
+*)
+
+Import BigStep.
+
+
+
+
+
+
+Section EnvironmentLemmas_GetValue.
+
+
+
+  Lemma get_value_singleton :
+    forall Γ key vs,
+        get_value Γ key = Some vs
+    ->  exists value, vs = [value].
+  Proof.
+    intros Γ key vs.
+     induction Γ as [| [k v] Γ IH]; intros Hget; cbn in Hget.
+     * congruence.
+     * destruct (var_funid_eqb key k) eqn:Heqb.
+       - exists v.
+         by inv Hget.
+       - by apply IH.
+  Qed.
+
+
+
+  Lemma get_value_singleton_length :
+    forall Γ key l,
+        get_value Γ key = Some l
+    ->  length l = 1.
+  Proof.
+    (* #1 Pose by Previous: intro/pose/inversion *)
+    itr - Γ key vs Hget.
+    pse - get_value_singleton as Hsingl: Γ key vs Hget.
+    bvs - Hsingl.
+  Qed.
+
+
+
+  Lemma get_value_single_det :
+    forall k1 k2 v1 v2,
+        get_value [(k1, v1)] k2 = Some [v2]
+    ->  k1 = k2 /\  v1 = v2.
+  Proof.
+    itr - k1 k2 v1 v2 Hget.
+    smp - Hget.
+    des > (var_funid_eqb k2 k1) as Hk; ivc - Hget.
+    spl.
+    2: rfl.
+    ufl - var_funid_eqb in Hk.
+    des - k1 as [s1 | f1]; des - k2 as [s2 | f2]; smp - Hk.
+    * app - String.eqb_eq in Hk.
+      bvs - Hk.
+    * con.
+    * con.
+    * ufl - funid_eqb in Hk.
+      des - f1 as [i1 n1]; des - f2 as [i2 n2]; smp - Hk.
+      app - andb_prop in Hk.
+      des - Hk as [Hi Hn].
+      app - String.eqb_eq in Hi.
+      app - Nat.eqb_eq in Hn.
+      sbt.
+      rfl.
+  Qed.
+
+
+
+  Lemma get_value_cons :
+    forall Γ key k var v,
+        get_value ((k, v) :: Γ) key = Some [var]
+    ->  get_value [(k, v)] key = Some [var] 
+    \/  get_value Γ key = Some [var].
+  Proof.
+    (* #1 Destruct Key Equality: intro/simpl/destruct/auto *)
+    itr - Γ key k var v Hcons.
+    smp *.
+    des > (var_funid_eqb key k) as Heqb_key; ato.
+  Qed.
+
+
+
+  Theorem get_value_in :
+    forall Γ key var,
+        get_value Γ key = Some [var]
+    ->  In (key , var) Γ.
+  Proof.
+    (* #1 Induction on Environment: intro/induction + intro/inversion *)
+    itr - Γ.
+    ind - Γ as [| [k v] Γ IH] :> itr - key var Hget :- ivc - Hget.
+    (* #2 Destruct Get_Value: apply/destruct *)
+    app - get_value_cons in Hget.
+    des - Hget as [Hget | Hget].
+    * (* #3.1 Destruct Key Equality: clear/simpl/destruct + congruence *)
+      clr - IH.
+      smp *.
+      des > (var_funid_eqb key k) as Hkey :- con.
+      (* #4.1 Rewrite Var & FunId: left/inversion/apply/rewrite *)
+      lft.
+      ivc - Hget.
+      app - var_funid_eqb_eq in Hkey.
+      bwr - Hkey.
+    * (* #3.2 Pose In_Cons: specialize/pose *)
+      spc - IH: key var Hget.
+      by pose proof in_cons (k, v) (key, var) Γ IH.
+  Qed.
+
+
+
+End EnvironmentLemmas_GetValue.
+
+
+
+
+
+
+
+
+
+Section EnvironmentLemmas_Remove.
+
+
+
+  Lemma rem_keys_empty :
+    forall Γ,
+      rem_keys [] Γ = Γ.
+  Proof.
+    (* #1 Induction on Environment: induction + simpl*)
+    ind - Γ as [| [k v] Γ IH] :> smp.
+    (* #2 Rewrite by Induction: rewrite *)
+    bwr - IH.
+  Qed.
+
+
+
+  Lemma rem_ext_empty :
+    forall Γ,
+      rem_ext [] Γ = Γ.
+  Proof.
+    app - rem_keys_empty.
+  Qed.
+
+
+
+End EnvironmentLemmas_Remove.
+
+
+
+
+
+
+
+
+
+
+
+
+(*
+////////////////////////////////////////////////////////////////////////////////
+//// CHAPTER: ERASER_SUBST_APPEND //////////////////////////////////////////////
+////////////////////////////////////////////////////////////////////////////////
+*)
+
+
+
+Section EraserSubstAppend_EraserLemmas.
+
+
+
+  Lemma add_keys_app :
+    forall keys1 keys2 σ,
+      add_keys keys1 (add_keys keys2 σ)
+    = add_keys (keys1 ++ keys2) σ.
+  Proof.
+    itr.
+    ufl - add_keys.
+    unfold add_names.
+    bwr - foldr_app.
+  Qed.
+
+
+
+  Lemma add_keys_get_env_app :
+    forall ext Γ σ,
+        add_keys (map fst (get_env Γ ext)) σ
+      = add_ext ext (add_keys (map fst Γ) σ).
+  Proof.
+    itr - ext Γ σ.
+    ufl - get_env.
+    rwr - map_app.
+    rwr - ext_to_env_fst.
+    rwl - add_keys_app.
+    ufl - add_ext add_fids.
+    bwr - map_map.
+  Qed.
+
+
+
+  Lemma add_keys_append_vars_to_env_app :
+    forall vars vs Γ σ,
+        length vars = length vs
+    ->  add_keys (map fst (append_vars_to_env vars vs Γ)) σ
+      = add_vars vars (add_keys (map fst Γ) σ).
+  Proof.
+    itr - vars vs Γ σ Hlength.
+    ufl - append_vars_to_env.
+    rwr - map_app.
+    rwl - add_keys_app.
+    epose proof length_map (inl : Var -> (Var + FunctionIdentifier)) vars
+      as Hlength_map_inl.
+    cwl - Hlength_map_inl in Hlength.
+    epose proof zip_fst _ _ _ _ Hlength as Hzip_fst;
+      clr - Hlength.
+    cwr - Hzip_fst.
+    ufl - add_vars.
+    trv.
+  Qed.
+
+
+
+  Lemma add_keys_append_vars_to_env_get_env_app :
+    forall vars vs ext Γ σ,
+        length vars = length vs
+    ->  add_keys (map fst (append_vars_to_env vars vs (get_env Γ ext))) σ
+      = add_vars vars (add_ext ext (add_keys (map fst Γ) σ)).
+  Proof.
+    itr - vars vs ext Γ σ Hlength.
+    rwr - add_keys_append_vars_to_env_app.
+    2: asm.
+    bwr - add_keys_get_env_app.
+  Qed.
+
+
+
+  Lemma add_keys_append_funs_to_env_app :
+    forall ext n Γ σ,
+        add_keys (map fst (append_funs_to_env ext Γ n)) σ
+      = add_fids (map fst ext) (add_keys (map fst Γ) σ).
+  Proof.
+    itr - ext n Γ σ.
+    ufl - append_funs_to_env.
+    rwr - add_keys_get_env_app.
+    ufl - add_ext.
+    feq.
+    gen - n.
+    ind - ext as [| [fid [vars e]] ext IH]: smp.
+    itr.
+    smp.
+    feq.
+    bpe - IH: (S n).
+  Qed.
+
+
+End EraserSubstAppend_EraserLemmas.
+
+
+
+
+
+
+
+
+
+Section EraserSubstAppend_SubstLemmas.
+
+
+
+  Lemma list_subst_cons :
+    forall v vs ξ,
+      list_subst [v] (list_subst vs ξ)
+    = list_subst (v::vs) ξ.
+  Proof.
+    trv.
+  Qed.
+
+
+
+  Lemma list_subst_fold_right :
+    forall vs ξ,
+      fold_right (fun v σ => v .: σ) ξ vs
+    = list_subst vs ξ.
+  Proof.
+    trv.
+  Qed.
+
+
+
+  Lemma list_subst_app :
+    forall vs1 vs2 ξ,
+      list_subst vs1 (list_subst vs2 ξ)
+    = list_subst (vs1 ++ vs2) ξ.
+  Proof.
+    itr.
+    rewrite <- list_subst_fold_right with (vs:= vs1 ++ vs2).
+    rewrite <- list_subst_fold_right with (vs:= vs1).
+    rewrite <- list_subst_fold_right with (vs:= vs2).
+    bwr - foldr_app.
+  Qed.
+
+
+
+End EraserSubstAppend_SubstLemmas.
+
+
+
+
+
+
+
+
+
+Section EraserSubstAppend_Theorems.
+
+
+
+  Theorem erase_exp_append_vars :
+    forall e fns env vars vs,
+        base.length vars = base.length vs
+    ->  (erase_exp
+          (add_keys
+            (map fst (append_vars_to_env vars vs env))
+            fns)
+          e)
+        .[list_subst
+          (map
+            (fun v => erase_val (measure_val v) fns v)
+            (map snd (append_vars_to_env vars vs env)))
+          idsubst]
+      = (erase_exp
+          (add_vars
+            vars
+            (add_keys (map fst env) fns))
+          e)
+        .[upn
+          (base.length vars)
+          (list_subst
+            (map
+               (fun v =>
+                 erase_val 
+                 (measure_val v) fns v)
+               (map snd env)) idsubst)]
+        .[list_subst
+          (map
+            (fun v => erase_val (measure_val v) fns v) vs)
+            idsubst].
+  Proof.
+    itr - e fns env vars vs Hlength.
+    (* add_keys *)
+    rwr - add_keys_append_vars_to_env_app.
+    (* upn to ++ *)
+    rwr - subst_comp_exp.
+    ass >
+      (length vs
+        = length (map (λ v : Value, erase_val (measure_val v) fns v) vs))
+      as Hlength_vars:
+      rwr - length_map.
+    rwl - Hlength in Hlength_vars.
+    cwr - Hlength_vars.
+    rwr - substcomp_list.
+    rwr - substcomp_id_l.
+    rwr - list_subst_app.
+    (* append to ++ *)
+    ufl - append_vars_to_env.
+    rwr - map_app.
+    epose proof length_map (inl : Var -> (Var + FunctionIdentifier)) vars
+      as Hlength_map_inl.
+    2: asm.
+    cwl - Hlength_map_inl in Hlength.
+    epose proof zip_snd _ _ _ _ Hlength as Hzip_snd;
+      clr - Hlength.
+    rwr - Hzip_snd.
+    bwr - map_app.
+  Qed.
+
+
+
+End EraserSubstAppend_Theorems.
+
+
+
+
+
+
+
+
+
+
+
+
+(*
+////////////////////////////////////////////////////////////////////////////////
+//// CHAPTER: MEASURE_VALUE ////////////////////////////////////////////////////
+////////////////////////////////////////////////////////////////////////////////
+*)
+
+
+Section tmp.
+End tmp.
+
+
+
+
+
+
+
+
+
+
+
+
+(*
+////////////////////////////////////////////////////////////////////////////////
+//// CHAPTER: MEASURE_VALUE ////////////////////////////////////////////////////
+////////////////////////////////////////////////////////////////////////////////
+*)
+
+
+Section tmp.
+End tmp.
+
+
+
+
+
+
+
+
+
+
+
+
+(*
+////////////////////////////////////////////////////////////////////////////////
+//// CHAPTER: MEASURE_VALUE ////////////////////////////////////////////////////
+////////////////////////////////////////////////////////////////////////////////
+*)
+
+
+Section tmp.
+End tmp.
+
+
+
+
+
+
+
+
+
+
+
+
+(*
+////////////////////////////////////////////////////////////////////////////////
+//// CHAPTER: MEASURE_VALUE ////////////////////////////////////////////////////
+////////////////////////////////////////////////////////////////////////////////
+*)
+
+
+Section tmp.
+End tmp.
+
+
+
+
+
+
+
+
+
+
+
+
+(*
+////////////////////////////////////////////////////////////////////////////////
+//// CHAPTER: MEASURE_VALUE ////////////////////////////////////////////////////
+////////////////////////////////////////////////////////////////////////////////
+*)
+
+
+Section tmp.
+End tmp.
