src/Eqvivalence/Tactics/T1ParamZero.v
@@ -1,0 +1,61 @@
+Require Import Coq.micromega.Lia.
+Require Import stdpp.list.
+
+
+
+(** DOCUMENTATION:
+
+* rfl --> reflexivity
+* asm --> assumption
+* dis --> discriminate
+* con --> congruence
+* spl --> split
+* lft --> left
+* rgt --> right
+* sbt --> subst
+* trv --> trivial
+* ato --> auto
+* tau --> tauto
+* itu --> intuition
+* fro --> firstorder
+* feq --> f_equal
+* ceq --> case_eq
+* adm --> admit.
+* sli --> simpl; lia
+* cli --> cbn; nia
+* sni --> simpl; cia
+* cni --> cbn; nia
+
+UNSGHANGED:
+* lia, nia, cut
+*)
+
+
+
+
+
+
+Ltac rfl := reflexivity.
+Ltac asm := assumption.
+Ltac dis := discriminate.
+Ltac con := congruence.
+Ltac spl := split.
+Ltac lft := left.
+Ltac rgt := right.
+Ltac sbt := subst.
+Ltac trv := trivial.
+Ltac ato := auto.
+Ltac tau := tauto.
+Ltac itu := intuition.
+Ltac fro := firstorder.
+Ltac feq := f_equal.
+Ltac ceq := case_eq.
+Ltac adm := admit.
+
+
+
+Ltac sli := simpl; lia.
+Ltac cli := cbn; lia.
+
+Ltac sni := simpl; nia.
+Ltac cni := cbn; nia.
