src/Eqvivalence/WellFormedMap.v
@@ -1,0 +1,148 @@
+From CoreErlang.BigStep Require BigStep.
+From CoreErlang Require SubstSemantics.
+From CoreErlang Require Basics.
+Require Import stdpp.list.
+
+(** CONTENT:
+* WELLFORMEDMAP_BIGSTEP
+  - WellFormedMap_BigStep_Value
+    + wfm_bs_val
+* WELLFORMEDMAP_FRAMESTACK
+  -WellFormedMap_FrameStack_Value
+    + wfm_fs_val
+*)
+
+
+
+
+
+
+
+
+
+
+
+
+(*
+////////////////////////////////////////////////////////////////////////////////
+//// CHAPTER: WELLFORMEDMAP_BIGSTEP ////////////////////////////////////////////
+////////////////////////////////////////////////////////////////////////////////
+*)
+
+Import BigStep.
+Import Basics.
+
+
+
+
+
+
+Section WellFormedMap_BigStep_Value.
+
+
+
+  Fixpoint wfm_bs_val
+      (v : Value)
+      : Prop
+      :=
+    match v with
+    | VCons hd tl =>
+        wfm_bs_val hd
+        /\
+        wfm_bs_val tl
+
+    | VTuple l =>
+        fold_right
+          (fun v acc =>
+            wfm_bs_val v /\ acc)
+          True
+          l
+
+    | VClos env _ _ _ _ =>
+        fold_right
+          (fun kv acc =>
+            wfm_bs_val (snd kv) /\ acc)
+          True
+          env
+
+    | VMap l =>
+        (l =
+        let (kl , vl) :=
+          (make_value_map
+            (fst (split l))
+            (snd (split l)))
+        in zip kl vl)
+        /\
+        fold_right
+          (fun v acc =>
+            PBoth wfm_bs_val v /\ acc)
+          True
+          l
+
+    | _ => True
+    end.
+
+
+
+End WellFormedMap_BigStep_Value.
+
+
+
+
+
+
+
+
+
+
+
+
+(*
+////////////////////////////////////////////////////////////////////////////////
+//// CHAPTER: WELLFORMEDMAP_FRAMESTACK /////////////////////////////////////////
+////////////////////////////////////////////////////////////////////////////////
+*)
+
+Import SubstSemantics.
+
+
+
+
+
+
+Section WellFormedMap_FrameStack_Value.
+
+
+
+  Fixpoint wfm_fs_val
+      (v : Val)
+      : Prop
+      :=
+    match v with
+
+    | VCons hd tl =>
+        wfm_fs_val hd
+      /\
+        wfm_fs_val tl
+
+    | VTuple l =>
+        fold_right
+          (fun v acc => wfm_fs_val v /\ acc)
+          True
+          l
+
+    | VMap l =>
+        l = make_val_map l
+      /\
+        fold_right
+          (fun v acc => PBoth wfm_fs_val v /\ acc)
+          True
+          l
+
+    | _ => True
+
+    end.
+
+
+
+End WellFormedMap_FrameStack_Value.
